src/Examples/HACMSDemo/WheelSensor.v
@@ -17,6 +17,7 @@ Require Import
 
 Require Import
         Fiat.Common.SumType
+        Fiat.Examples.DnsServer.DecomposeEnumField
         Fiat.QueryStructure.Automation.AutoDB
         Fiat.QueryStructure.Implementation.DataStructures.BagADT.BagADT
         Fiat.QueryStructure.Automation.IndexSelection
@@ -48,6 +49,156 @@ Definition IPAddress := word 32.
 Definition SensorTypeCode : Vector.t (word 4) 2
   := [ natToWord 4 3; natToWord 4 0].
 
+Fixpoint BuildFinUpTo (n : nat) {struct n} : list (Fin.t n) :=
+  match n return list (Fin.t n) with
+  | 0  => nil
+  | S n' => cons (@Fin.F1 _) (map (@Fin.FS _) (BuildFinUpTo n'))
+  end.
+
+Definition allAttributes heading
+  : list (Attributes heading) :=
+  BuildFinUpTo (NumAttr heading).
+
+Lemma agreeAllAttributes_eq
+  : forall heading tup tup',
+    tupleAgree_computational tup tup'
+                             (allAttributes heading) <-> tup = tup'.
+Proof.
+  destruct heading.
+  induction AttrList; unfold RawTuple; simpl; intros.
+  - destruct tup; destruct tup'; intuition.
+  - destruct tup; destruct tup'; simpl.
+    intuition.
+    + unfold GetAttributeRaw in H0; simpl in H0; unfold ilist2_hd in H0;
+      simpl in H0; subst.
+      unfold allAttributes in IHAttrList.
+      rewrite (proj1 (IHAttrList prim_snd prim_snd0)); eauto; simpl.
+      revert H1.
+      induction (BuildFinUpTo n); simpl; intuition.
+    + injections; eauto.
+    + injections.
+      generalize (proj2 (IHAttrList prim_snd0 prim_snd0) eq_refl); clear.
+      induction (BuildFinUpTo n); simpl; intuition.
+Qed.
+
+Lemma refine_DuplicateFree
+      {qsSchema}
+  : forall (qs : UnConstrQueryStructure qsSchema) Ridx tup',
+    (forall tup , tup = tup' \/ tup <> tup')
+    -> refine
+      {b : bool |
+       decides b
+               (forall tup : IndexedElement,
+                   GetUnConstrRelation qs Ridx tup ->
+                   DuplicateFree tup' (indexedElement tup))}
+      (xs <- For (UnConstrQuery_In qs Ridx
+                           (fun tup => Where (tupleAgree_computational tup tup' (allAttributes _) )
+                                             Return tup));
+       ret (If_Opt_Then_Else (hd_error xs) (fun _ => false) true)).
+Proof.
+  unfold refine; intros.
+  computes_to_inv; subst.
+  destruct v0; simpl; computes_to_econstructor; simpl; intros.
+  unfold not; intro.
+  unfold UnConstrQuery_In in H0; simpl; subst.
+  apply (For_computes_to_nil (fun tup0 => (tupleAgree_computational tup0
+                                                                    (indexedElement tup)
+                        (allAttributes
+                           (GetNRelSchemaHeading (qschemaSchemas qsSchema)
+                              Ridx)))) _ H0 _ H1).
+  apply agreeAllAttributes_eq; eauto.
+  intro.
+  apply For_computes_to_In with (x := r) in H0; intuition.
+  destruct_ex; intuition; subst.
+  apply H1 in H3.
+  apply agreeAllAttributes_eq in H2; unfold DuplicateFree in *.
+  rewrite <- H2 in H3; apply H3; reflexivity.
+  rewrite agreeAllAttributes_eq; eapply (H a).
+Qed.
+
+Lemma DeleteDuplicateFreeOK {qsSchema}
+  : forall (qs : UnConstrQueryStructure qsSchema)
+           (Ridx :Fin.t _)
+           DeletedTuples,
+      refine {b | (forall tup tup',
+                      elementIndex tup <> elementIndex tup'
+                      -> GetUnConstrRelation qs Ridx tup
+                      -> GetUnConstrRelation qs Ridx tup'
+                      -> (DuplicateFree (indexedElement tup) (indexedElement tup')))
+                  -> decides b (Mutate.MutationPreservesTupleConstraints
+                                  (EnsembleDelete (GetUnConstrRelation qs Ridx) DeletedTuples)
+                                  DuplicateFree
+             )}
+             (ret true).
+Proof.
+  unfold Mutate.MutationPreservesTupleConstraints, DuplicateFree;
+  intros * v Comp_v;  computes_to_inv; subst.
+  computes_to_constructor; simpl.
+  intros.
+  unfold EnsembleDelete in *; destruct H1; destruct H2; eauto.
+Qed.
+
+Lemma refine_DuplicateFree_symmetry
+      {qsSchema}
+  : forall (qs : UnConstrQueryStructure qsSchema) Ridx tup' b',
+    computes_to {b : bool | decides b
+                                     (forall tup : IndexedElement,
+                                         GetUnConstrRelation qs Ridx tup ->
+                                         DuplicateFree tup' (indexedElement tup)  )} b'
+    -> refine
+         {b : bool |
+          decides b
+                  (forall tup : IndexedElement,
+                      GetUnConstrRelation qs Ridx tup ->
+                      DuplicateFree (indexedElement tup) tup')}
+         (ret b').
+Proof.
+  intros.
+  repeat computes_to_inv; computes_to_econstructor.
+  computes_to_inv; subst.
+  destruct v; simpl in *; unfold DuplicateFree in *; intros.
+  intuition eauto.
+  intuition eauto.
+Qed.
+
+Ltac implement_DuplicateFree :=
+  match goal with
+    |- context [{b : bool |
+                 decides b
+                         (forall tup' : IndexedElement,
+                             GetUnConstrRelation ?r ?Ridx tup' ->
+                                 DuplicateFree ?tup (indexedElement tup'))}] =>
+    rewrite (@refine_DuplicateFree _ r Ridx); [ | intros; repeat decide equality]
+  end.
+
+Ltac implement_DuplicateFree_symmetry :=
+  match goal with
+    |- context [{b : bool |
+                 decides b
+                         (forall tup' : IndexedElement,
+                             GetUnConstrRelation ?r ?Ridx tup' ->
+                                 DuplicateFree  (indexedElement tup') ?tup)}] =>
+    rewrite (@refine_DuplicateFree_symmetry _ r Ridx)
+  end.
+
+Ltac RemoveDeleteDuplicateFreeCheck :=
+    match goal with
+        |- context[{b | (forall tup tup',
+                           elementIndex tup <> elementIndex tup'
+                           -> GetUnConstrRelation ?qs ?Ridx tup
+                           -> GetUnConstrRelation ?qs ?Ridx tup'
+                           -> (DuplicateFree (indexedElement tup) (indexedElement tup')))
+                        -> decides b (Mutate.MutationPreservesTupleConstraints
+                                        (EnsembleDelete (GetUnConstrRelation ?qs ?Ridx) ?DeletedTuples)
+                                        DuplicateFree
+                                     )}] =>
+        let refinePK := fresh in
+        pose proof (DeleteDuplicateFreeOK qs Ridx DeletedTuples) as refinePK;
+          simpl in refinePK; pose_string_hyps_in refinePK; pose_heading_hyps_in refinePK;
+          setoid_rewrite refinePK; clear refinePK;
+          try setoid_rewrite refineEquiv_bind_unit
+    end.
+
 Variable cache : Cache.
 Variable cacheAddNat : CacheAdd cache nat.
 Definition transformer : Transformer bin := btransformer.
@@ -68,7 +219,7 @@ Definition encode_SensorData_Spec (val : SensorType) :=
 Definition WheelSensorSchema :=
   Query Structure Schema
     [ relation "subscribers" has
-               schema <"address" :: IPAddress, "topic" :: SensorID>
+               schema <"topic" :: SensorID, "address" :: IPAddress>
       where DuplicateFree
     ] enforcing [ ].
 
@@ -90,8 +241,8 @@ Definition WheelSensorSig : ADTSig :=
       Constructor "Init" : rep,
       Method "AddSpeedSubscriber" : rep * IPAddress -> rep * bool,
       Method "AddTirePressureSubscriber" : rep * IPAddress -> rep * bool,
-      Method "PublishSpeed" : rep * nat -> rep * (list bin),
-      Method "PublishTirePressure" : rep * nat -> rep * (list bin)
+      Method "PublishSpeed" : rep * nat -> rep * (list (IPAddress * bin)),
+      Method "PublishTirePressure" : rep * nat -> rep * (list (IPAddress * bin))
     }.
 
 (* Now we write what the methods should actually do. *)
@@ -106,23 +257,282 @@ Definition WheelSensorSpec : ADT WheelSensorSig :=
     Def Constructor0 "Init" : rep := empty,,
 
     Def Method1 "AddSpeedSubscriber" (r : rep) (addr : IPAddress) : rep * bool :=
-        Insert <"address" :: addr, "topic" :: ``"Speed"> into r!"subscribers",
+        Insert <"topic" :: ``"Speed", "address" :: addr> into r!"subscribers",
 
     Def Method1 "AddTirePressureSubscriber" (r : rep) (addr : IPAddress) : rep * bool :=
-        Insert <"address" :: addr, "topic" :: ``"TirePressure"> into r!"subscribers",
+        Insert <"topic" :: ``"TirePressure", "address" :: addr> into r!"subscribers",
 
-    Def Method1 "PublishSpeed" (r : rep) (n : nat) : rep * (list bin) :=
+    Def Method1 "PublishSpeed" (r : rep) (n : nat) : rep * (list (IPAddress* bin)) :=
+          `(msg, _) <- encode_SensorData_Spec (inj_SumType SensorTypes SensorIDs[@"Speed"] n) Empty;
           subs <- For (sub in r!"subscribers")
-                    Where (sub!"topic" = ``"Speed")
-                    (l <- encode_SensorData_Spec (inj_SumType SensorTypes SensorIDs[@"Speed"] n) Empty;
-                     Return (fst l));
+                  Where (sub!"topic" = ``"Speed")
+                  Return (sub!"address", msg);
           ret (r, subs),
 
-    Def Method1 "PublishTirePressure" (r : rep) (n : nat) : rep * (list bin) :=
+    Def Method1 "PublishTirePressure" (r : rep) (n : nat) : rep * (list (IPAddress * bin)) :=
+          `(msg, _) <- encode_SensorData_Spec (inj_SumType SensorTypes SensorIDs[@"TirePressure"] n) Empty;
           subs <- For (sub in r!"subscribers")
-                    Where (sub!"topic" = ``"TirePressure")
-                    (l <- encode_SensorData_Spec (inj_SumType SensorTypes SensorIDs[@"TirePressure"] n)
- Empty;
-                     Return (fst l));
+                  Where (sub!"topic" = ``"TirePressure")
+                  Return (sub!"address", msg);
           ret (r, subs)
   }%methDefParsing.
+
+Lemma refineEquiv_Query_Where_And
+      {ResultT}
+  : forall P P' bod,
+    (P \/ ~ P)
+    -> refineEquiv (@Query_Where ResultT (P /\ P') bod)
+                (Query_Where P (Query_Where P' bod)).
+Proof.
+  split; unfold refine, Query_Where; intros;
+    computes_to_inv; computes_to_econstructor;
+      intuition.
+  - computes_to_inv; intuition.
+  - computes_to_inv; intuition.
+  - computes_to_econstructor; intuition.
+Qed.
+
+Corollary refineEquiv_For_Query_Where_And
+          {ResultT}
+          {qs_schema}
+  : forall (r : UnConstrQueryStructure qs_schema) idx P P' bod,
+    (forall tup, P tup \/ ~ P tup)
+    -> refine (For (UnConstrQuery_In
+                      r idx
+                      (fun tup => @Query_Where ResultT (P tup /\ P' tup) (bod tup))))
+              (For (UnConstrQuery_In
+                      r idx
+                      (fun tup => Where (P tup) (Where (P' tup) (bod tup))))).
+Proof.
+  intros; apply refine_refine_For_Proper.
+  apply refine_UnConstrQuery_In_Proper.
+  intro; apply refineEquiv_Query_Where_And; eauto.
+Qed.
+
+Lemma IPAddress_decideable
+  : forall (addr addr' : IPAddress),
+    (addr = addr') \/ (addr <> addr').
+Proof.
+  intros; destruct (weq addr addr'); intuition.
+Qed.
+
+Lemma SensorID_decideable
+  : forall (id1 id2 : SensorID),
+    (id1 = id2) \/ (id1 <> id2).
+Proof.
+  intros; destruct (BoundedIndex_eq_dec id1 id2); intuition.
+Qed.
+
+Lemma refine_If_IfOpt {A B}
+  : forall (a_opt : option A) (t e : Comp B),
+    refine (If_Then_Else (If_Opt_Then_Else a_opt (fun _ => false) true)
+                         t e)
+           (If_Opt_Then_Else a_opt (fun _ => e) t).
+Proof.
+  destruct a_opt; simpl; intros; reflexivity.
+Qed.
+
+Theorem SharpenedWheelSensor :
+  FullySharpened WheelSensorSpec.
+Proof.
+  start sharpening ADT.
+  start_honing_QueryStructure'.
+  hone method "AddSpeedSubscriber".
+  { simplify with monad laws.
+    etransitivity.
+    eapply refine_under_bind; intros.
+    implement_DuplicateFree;
+      try first [eapply IPAddress_decideable | eapply SensorID_decideable].
+    eapply refine_under_bind; intros.
+    implement_DuplicateFree_symmetry; eauto;
+    [ | apply refine_DuplicateFree; eauto ].
+    simplify with monad laws.
+    set_evars.
+    rewrite !refine_if_If.
+    rewrite refine_If_Then_Else_Duplicate.
+    setoid_rewrite refine_pick_eq'; simplify with monad laws.
+    finish honing.
+    intros; repeat decide equality;
+      first [eapply IPAddress_decideable | eapply SensorID_decideable].
+    simpl; simplify with monad laws.
+    subst; finish honing.
+  }
+  hone method "AddTirePressureSubscriber".
+  { simplify with monad laws.
+    etransitivity.
+    eapply refine_under_bind; intros.
+    implement_DuplicateFree;
+      try first [eapply IPAddress_decideable | eapply SensorID_decideable].
+    eapply refine_under_bind; intros.
+    implement_DuplicateFree_symmetry; eauto;
+    [ | apply refine_DuplicateFree; eauto ].
+    simplify with monad laws.
+    set_evars.
+    rewrite !refine_if_If.
+    rewrite refine_If_Then_Else_Duplicate.
+    setoid_rewrite refine_pick_eq'; simplify with monad laws.
+    finish honing.
+    intros; repeat decide equality;
+      first [eapply IPAddress_decideable | eapply SensorID_decideable].
+    simpl; simplify with monad laws.
+    subst; finish honing.
+  }
+  let AbsR' := constr:(@DecomposeRawQueryStructureSchema_AbsR' 2 WheelSensorSchema ``"subscribers" ``"topic" id (fun i => ibound (indexb i))
+                                                (fun val =>
+                                                   {| bindex := _;
+                                                      indexb := {| ibound := val;
+                                                                   boundi := @eq_refl _ _ |} |})) in hone representation using AbsR'.
+  {
+    simplify with monad laws.
+    apply refine_pick_val.
+    apply DecomposeRawQueryStructureSchema_empty_AbsR.
+  }
+  {
+    simplify with monad laws.
+    etransitivity.
+    apply refine_under_bind_both; intros.
+    apply (refine_UnConstrFreshIdx_DecomposeRawQueryStructureSchema_AbsR_Equiv H0 Fin.F1).
+    apply refine_under_bind_both; intros.
+    etransitivity.
+    eapply (refineEquiv_For_Query_Where_And r_o Fin.F1).
+    intros; eapply SensorID_decideable.
+    simpl.
+    setoid_rewrite (@refine_QueryIn_Where _ WheelSensorSchema Fin.F1 _ _ _ _ _ H0 _ _ _ ).
+    unfold Tuple_DecomposeRawQueryStructure_inj; simpl.
+    reflexivity.
+    rewrite refine_If_IfOpt.
+    etransitivity.
+    eapply refine_If_Opt_Then_Else_Bind; simpl.
+    apply refine_If_Opt_Then_Else; unfold pointwise_relation; intros.
+    simplify with monad laws.
+    rewrite_drill.
+    apply refine_pick_val.
+    apply H0.
+    simpl; finish honing.
+    simplify with monad laws; simpl.
+    rewrite_drill.
+    apply refine_pick_val.
+    apply (DecomposeRawQueryStructureSchema_Insert_AbsR_eq H0).
+    finish honing.
+    simpl; finish honing.
+  }
+  {
+    simplify with monad laws.
+    etransitivity.
+    apply refine_under_bind_both; intros.
+    apply (refine_UnConstrFreshIdx_DecomposeRawQueryStructureSchema_AbsR_Equiv H0 Fin.F1).
+    apply refine_under_bind_both; intros.
+    etransitivity.
+    eapply (refineEquiv_For_Query_Where_And r_o Fin.F1).
+    intros; eapply SensorID_decideable.
+    simpl.
+    setoid_rewrite (@refine_QueryIn_Where _ WheelSensorSchema Fin.F1 _ _ _ _ _ H0 _ _ _ ).
+    unfold Tuple_DecomposeRawQueryStructure_inj; simpl.
+    reflexivity.
+    rewrite refine_If_IfOpt.
+    etransitivity.
+    eapply refine_If_Opt_Then_Else_Bind; simpl.
+    apply refine_If_Opt_Then_Else; unfold pointwise_relation; intros.
+    simplify with monad laws.
+    rewrite_drill.
+    apply refine_pick_val.
+    apply H0.
+    simpl; finish honing.
+    simplify with monad laws; simpl.
+    rewrite_drill.
+    apply refine_pick_val.
+    apply (DecomposeRawQueryStructureSchema_Insert_AbsR_eq H0).
+    finish honing.
+    simpl; finish honing.
+  }
+  {
+    simplify with monad laws.
+    rewrite_drill.
+    setoid_rewrite (@refine_QueryIn_Where _ WheelSensorSchema Fin.F1 _ _ _ _ _ H0 _ _ _ ).
+    unfold Tuple_DecomposeRawQueryStructure_inj; simpl.
+    finish honing.
+    rewrite_drill.
+    apply refine_pick_val; eassumption.
+    simpl.
+    finish honing.
+  }
+  { simplify with monad laws.
+    rewrite_drill.
+    setoid_rewrite (@refine_QueryIn_Where _ WheelSensorSchema Fin.F1 _ _ _ _ _ H0 _ _ _ ).
+    unfold Tuple_DecomposeRawQueryStructure_inj; simpl.
+    finish honing.
+    rewrite_drill.
+    apply refine_pick_val; eassumption.
+    simpl.
+    finish honing.
+  }
+  hone representation using (fun r_o r_n => snd r_o = r_n).
+  { simplify with monad laws.
+    apply refine_pick_val.
+    reflexivity.
+  }
+  { simplify with monad laws.
+    rewrite H0.
+    rewrite_drill; try (clear r_o H0; finish honing).
+    rewrite_drill; try (clear r_o H0; finish honing).
+    etransitivity.
+    apply refine_If_Opt_Then_Else_Bind.
+    unfold H2; eapply refine_If_Opt_Then_Else.
+    intro; simplify with monad laws.
+    apply refine_bind.
+    apply refine_pick_val; eauto.
+    intro; simpl; finish honing.
+    simplify with monad laws.
+    simpl; apply refine_bind.
+    apply refine_pick_val; eauto.
+    intro; simpl; finish honing.
+  }
+  { simplify with monad laws.
+    rewrite H0.
+    rewrite_drill; try (clear r_o H0; finish honing).
+    rewrite_drill; try (clear r_o H0; finish honing).
+    etransitivity.
+    apply refine_If_Opt_Then_Else_Bind.
+    unfold H2; eapply refine_If_Opt_Then_Else.
+    intro; simplify with monad laws.
+    apply refine_bind.
+    apply refine_pick_val; eauto.
+    intro; simpl; finish honing.
+    simplify with monad laws.
+    simpl; apply refine_bind.
+    apply refine_pick_val; eauto.
+    intro; simpl; finish honing.
+  }
+  { simplify with monad laws.
+    rewrite H0.
+    etransitivity.
+    apply refine_under_bind; intros.
+    simpl; apply refine_bind.
+    apply refine_pick_val; eauto.
+    intro; simpl; finish honing.
+    simpl. finish honing.
+  }
+  { simplify with monad laws.
+    rewrite H0.
+    etransitivity.
+    apply refine_under_bind; intros.
+    simpl; apply refine_bind.
+    apply refine_pick_val; eauto.
+    intro; simpl; finish honing.
+    simpl.
+    finish honing.
+  }
+  unfold  Tuple_DecomposeRawQueryStructure_proj; simpl.
+  unfold DecomposeRawQueryStructureSchema, DecomposeSchema; simpl.
+  let makeIndex attrlist :=
+      make_simple_indexes attrlist
+        ltac:(LastCombineCase6 BuildEarlyEqualityIndex)
+        ltac:(LastCombineCase5 BuildLastEqualityIndex) in
+  GenerateIndexesForAll EqExpressionAttributeCounter ltac:(fun attrlist =>
+                                                             let attrlist' := eval compute in (PickIndexes _ (CountAttributes' attrlist)) in makeIndex attrlist').
+  Require Import Fiat.Examples.Tutorial.Tutorial.
+  simplify with monad laws.
+  initializer.
+  - implement_insert CreateTerm EarlyIndex LastIndex
+                     makeClause_dep EarlyIndex_dep LastIndex_dep.
+    simplify with monad laws.
