src/Examples/DnsServer/DecomposeSumField.v
@@ -1,0 +1,775 @@
+Require Import
+        Coq.Vectors.Vector
+        Coq.Strings.Ascii
+        Coq.Bool.Bool
+        Coq.Lists.List.
+
+Require Import
+        Fiat.Common.SumType
+        Fiat.Computation.ListComputations
+        Fiat.QueryStructure.Automation.AutoDB
+        Fiat.Examples.DnsServer.Packet.
+
+Require Import
+        Bedrock.Word
+        Bedrock.Memory.
+
+
+Import Coq.Vectors.VectorDef.VectorNotations.
+
+Local Open Scope vector_scope.
+
+Section DecomposeEnumField.
+
+  (* Could use above to prove dependent inversion lemma, but *)
+  (* this is more of a sanity check than anything. *)
+  (* Lemma proj_SumType_inj_inverse {n}
+    : forall (v : Vector.t Type n)
+             (tag : Fin.t n)
+             (el : Vector.nth v tag),
+      SumType_proj v (inj_SumType v tag el) = el. *)
+
+  (* Goal: Convert from QueryStructure with a heading with a SumType *)
+  (* attribute to one that has multiple tables. *)
+  (* Is this a worthwhile refinement? We could just do this at data structure *)
+  (* selection time. OTOH, nice high-level refinement step that makes sense to *)
+  (* end-users and has applications in both DNS examples.  *)
+
+  Definition AddRawQueryStructureSchema
+             {m}
+             (raw_qs_schema : RawQueryStructureSchema)
+             (new_schemas : Vector.t RawSchema m)
+    : RawQueryStructureSchema :=
+    {| qschemaSchemas := Vector.append (qschemaSchemas raw_qs_schema) new_schemas;
+       qschemaConstraints := [ ] |}.
+
+  Fixpoint LiftTuple_AddRawQueryStructureSchema
+           {n m : nat}
+           (old_schemas : Vector.t RawSchema n)
+           (new_schemas : Vector.t RawSchema m)
+           Ridx
+           (tup : @RawTuple (GetNRelSchemaHeading old_schemas Ridx))
+           {struct old_schemas}
+    : @RawTuple
+        (GetNRelSchemaHeading (Vector.append old_schemas new_schemas)
+                              (Fin.L m Ridx)).
+    refine (match old_schemas in Vector.t _ n return
+                  forall (Ridx : Fin.t n),
+                    @RawTuple (GetNRelSchemaHeading old_schemas Ridx)
+                    -> @RawTuple
+                         (GetNRelSchemaHeading (Vector.append old_schemas new_schemas)
+                                               (Fin.L m Ridx)) with
+            | Vector.nil => fun Ridx tup => Fin.case0 (fun _ => _) Ridx
+            | Vector.cons _ _ _ => fun Ridx tup => _
+            end Ridx tup).
+    revert t tup0; pattern n0, Ridx0; apply Fin.caseS; simpl.
+    - intros; exact tup0.
+    - intros; exact (LiftTuple_AddRawQueryStructureSchema _ _ _ _ _ tup0).
+  Defined.
+
+  Definition AddRawQueryStructureSchema_AbsR
+             {m : nat}
+             {qs_schema : RawQueryStructureSchema}
+             (new_schemas : Vector.t RawSchema m)
+             (r_o : UnConstrQueryStructure qs_schema)
+             (r_n : UnConstrQueryStructure (AddRawQueryStructureSchema qs_schema new_schemas))
+    : Prop :=
+    (forall Ridx tup,
+        IndexedEnsemble_In (GetUnConstrRelation r_o Ridx) tup
+        <-> IndexedEnsemble_In (GetUnConstrRelation r_n (Fin.L m Ridx)) (LiftTuple_AddRawQueryStructureSchema _ _ Ridx tup)).
+
+  (* Define new schema *)
+
+  Fixpoint DecomposeHeading
+           {n m}
+           (attr : Fin.t n)
+           (sch : Vector.t Type n)
+           (a : Vector.t Type m)
+           {struct attr}
+    : Vector.t (Vector.t Type n) m :=
+    match attr in Fin.t n return Vector.t _ n ->  Vector.t (Vector.t _ n) m with
+    | Fin.F1 _ =>
+      fun sch =>
+        Vector.map (fun t => Vector.cons _ t _ (Vector.tl sch)) a
+    | Fin.FS _ attr' =>
+      fun sch =>
+        Vector.map (fun t => Vector.cons _ (Vector.hd sch) _ t)
+                   (DecomposeHeading attr' (Vector.tl sch) a)
+    end sch.
+
+  Fixpoint Tuple_mapHeading
+           {m q} {A' B' C}
+           (idx : Fin.t m)
+           (a : Vector.t C m)
+           (f : _ -> _ q)
+           (tup : ilist2 (A := A') (B := B') (Vector.map f a)[@idx])
+           {struct idx}
+    : ilist2 (B := B') (f a[@idx]).
+    refine (match idx in Fin.t m return
+                  forall (a : Vector.t C m)
+                         (f : _ -> _ q)
+                         (tup : ilist2 (B := B') (Vector.map f a)[@idx]),
+                    ilist2 (B := B') (f a[@idx]) with
+            | Fin.F1 _ => _
+            | Fin.FS _ idx' => _
+            end a f tup); clear a tup; intro; try revert idx';
+      pattern n, a; apply Vector.caseS.
+    - intros; exact tup.
+    - simpl; intros; eapply Tuple_mapHeading; eauto.
+  Defined.
+
+  Fixpoint Tuple_mapHeading_inv
+           {m q} {A' B' C}
+           (idx : Fin.t m)
+           (a : Vector.t C m)
+           (f : _ -> _ q)
+           (tup : ilist2 (B := B') (f a[@idx]))
+           {struct idx}
+    : ilist2 (A := A') (B := B') (Vector.map f a)[@idx].
+    refine (match idx in Fin.t m return
+                  forall (a : Vector.t C m)
+                         (f : _ -> _ q)
+                         (tup : ilist2 (B := B') (f a[@idx])),
+                    ilist2 (B := B') (Vector.map f a)[@idx] with
+            | Fin.F1 _ => _
+            | Fin.FS _ idx' => _
+            end a f tup); clear a tup; intro; try revert idx';
+      pattern n, a; apply Vector.caseS.
+    - intros; exact tup.
+    - simpl; intros; eapply Tuple_mapHeading_inv; eauto.
+  Defined.
+
+  Fixpoint Tuple_DecomposeHeading_inj
+           {n m}
+           (attrIdx : Fin.t n)
+           (heading : Vector.t Type n)
+           (a : Vector.t Type m)
+           (a_inj : forall idx, Vector.nth a idx -> Vector.nth heading attrIdx)
+           (idx : Fin.t m)
+           (tup : ilist2 (B := @id Type) (Vector.nth (DecomposeHeading attrIdx heading a) idx))
+           {struct attrIdx}
+    : ilist2 (B := @id Type) heading.
+    refine
+      (match attrIdx in Fin.t n return
+             forall (heading : Vector.t Type n)
+                    (a : Vector.t Type m)
+                    (a_inj : forall idx, Vector.nth a idx -> Vector.nth heading attrIdx)
+                    (idx : Fin.t m)
+                    (tup : ilist2 (B := @id Type) (Vector.nth (DecomposeHeading attrIdx heading a) idx)),
+               ilist2 (B := @id Type) heading with
+       | Fin.F1 _ => fun heading' => _
+       | Fin.FS _ attr' => fun heading' => _
+       end heading a a_inj idx tup).
+    - clear; pattern n0, heading'; eapply Vector.caseS.
+      simpl; intros.
+      exact (icons2 (B := @id Type)
+                    (a_inj idx (ilist2_hd (Tuple_mapHeading idx a _ tup)))
+                    (ilist2_tl (Tuple_mapHeading idx a _ tup))).
+    - revert attr'; pattern n0, heading'; eapply Vector.caseS.
+      simpl; intros.
+      exact (icons2
+               (ilist2_hd (Tuple_mapHeading _ _ _ tup0))
+               (Tuple_DecomposeHeading_inj
+                  _ _ attr' t _ a_inj0 _
+                  (ilist2_tl (Tuple_mapHeading _ _ _ tup0)))).
+  Defined.
+
+  Fixpoint Tuple_DecomposeHeading_proj
+           {n m}
+           (attrIdx : Fin.t n)
+           (heading : Vector.t Type n)
+           (a : Vector.t Type m)
+           (a_proj_index : Vector.nth heading attrIdx -> Fin.t m)
+           (a_proj : forall (attr : Vector.nth heading attrIdx),
+               a[@a_proj_index attr])
+           (tup : ilist2 (B := @id Type) heading)
+           {struct attrIdx}
+    : ilist2 (B := @id Type) (Vector.nth (DecomposeHeading attrIdx heading a) (a_proj_index (ith2 tup attrIdx))).
+    refine
+      (match attrIdx in Fin.t n return
+             forall
+               (heading : Vector.t Type n)
+               (a : Vector.t Type m)
+               (a_proj_index : Vector.nth heading attrIdx -> Fin.t m)
+               (a_proj : forall (attr : Vector.nth heading attrIdx),
+                   a[@a_proj_index attr])
+               (tup : ilist2 (B := @id Type) heading),
+               ilist2 (B := @id Type) (Vector.nth (DecomposeHeading attrIdx heading a) (a_proj_index (ith2 tup attrIdx))) with
+       | Fin.F1 _ => fun heading' => _
+       | Fin.FS _ attr' => fun heading' => _
+       end heading a a_proj_index a_proj tup).
+    - clear; pattern n0, heading'; eapply Vector.caseS.
+      simpl; intros.
+      exact (Tuple_mapHeading_inv
+               _ a _ (icons2 (B := @id Type) (a_proj (ilist2_hd tup)) (ilist2_tl tup))).
+    - revert attr'; pattern n0, heading'; eapply Vector.caseS.
+      simpl; intros.
+      refine (Tuple_mapHeading_inv
+                _ _ _
+                (icons2 (B := @id Type)
+                        (ilist2_hd tup0)
+                        (Tuple_DecomposeHeading_proj _ _ _ _ _ _ a_proj0 (ilist2_tl tup0)))).
+  Defined.
+
+  (* Could fuse this with Decompose Heading, but efficiency shouldn't matter too much. *)
+  Definition DecomposeSchema
+             {m}
+             (heading : RawSchema)
+             (attr : Fin.t _)
+             (a : Vector.t Type m)
+    : Vector.t RawSchema m :=
+    Vector.map
+      (fun rawheading =>
+         {| rawSchemaHeading := Build_RawHeading rawheading;
+            attrConstraints := None;
+            tupleConstraints := None |})
+      (DecomposeHeading attr (AttrList (rawSchemaHeading heading)) a).
+
+  Definition DecomposeRawQueryStructureSchema
+             {m}
+             (raw_qs_schema : RawQueryStructureSchema)
+             (schemaIdx : Fin.t _)
+             (attrIdx : Fin.t _)
+             (a : Vector.t Type m)
+    : RawQueryStructureSchema :=
+    {| qschemaSchemas :=
+         DecomposeSchema (Vector.nth (qschemaSchemas raw_qs_schema) schemaIdx)
+                         attrIdx a;
+       qschemaConstraints := [ ] |}.
+
+  Definition Tuple_DecomposeRawQueryStructure_proj
+             {m : nat}
+             {qs_schema : RawQueryStructureSchema}
+             (schemaIdx : Fin.t _)
+             (attrIdx : Fin.t _)
+             (a : Vector.t Type m)
+             (a_proj_index : Vector.nth (AttrList (GetNRelSchemaHeading (qschemaSchemas qs_schema) schemaIdx)) attrIdx -> Fin.t m)
+             (a_proj : forall (attr : Vector.nth _ attrIdx), a[@a_proj_index attr])
+             (tup : ilist2 (AttrList (GetNRelSchemaHeading (qschemaSchemas qs_schema) schemaIdx)))
+    :  ilist2 (B := @id Type) (AttrList (GetNRelSchemaHeading (qschemaSchemas (DecomposeRawQueryStructureSchema qs_schema schemaIdx attrIdx a)) (a_proj_index (GetAttributeRaw tup attrIdx)))).
+    unfold DecomposeRawQueryStructureSchema in *; simpl in *.
+    unfold GetNRelSchema, DecomposeSchema in *;
+      simpl in *.
+    erewrite VectorSpec.nth_map by eauto; simpl.
+    eapply Tuple_DecomposeHeading_proj; eauto.
+  Defined.
+
+  Definition Tuple_DecomposeRawQueryStructure_inj
+             {m : nat}
+             {qs_schema : RawQueryStructureSchema}
+             (schemaIdx : Fin.t _)
+             (attrIdx : Fin.t _)
+             (a : Vector.t Type m)
+             (a_inj : forall idx, Vector.nth a idx -> Vector.nth (AttrList (GetNRelSchemaHeading (qschemaSchemas qs_schema) schemaIdx)) attrIdx)
+             (idx : Fin.t m)
+             (tup : ilist2 (B := @id Type) (AttrList (GetNRelSchemaHeading (qschemaSchemas (DecomposeRawQueryStructureSchema qs_schema schemaIdx attrIdx a)) idx)))
+    : ilist2 (B := @id Type) (AttrList (GetNRelSchemaHeading (qschemaSchemas qs_schema) schemaIdx)).
+    unfold DecomposeRawQueryStructureSchema in *; simpl in *.
+    unfold GetNRelSchema, DecomposeSchema in *;
+      simpl in *.
+    erewrite VectorSpec.nth_map in tup by eauto; simpl.
+    simpl in tup.
+    eapply Tuple_DecomposeHeading_inj; eauto.
+  Defined.
+
+  Fixpoint Tuple_DecomposeRawQueryStructure_Tuple_inj
+             {n m : nat}
+             (headings : _ )
+             (idx : Fin.t m)
+             (tup : ilist2 (B := @id Type)
+          (AttrList
+             (rawSchemaHeading
+                (Vector.map
+                   (fun
+                      rawheading : t Type n =>
+                    {|
+                    rawSchemaHeading := {|
+                                        NumAttr := _;
+                                        AttrList := rawheading |};
+                    attrConstraints := None;
+                    tupleConstraints := None |})
+                   headings)[@idx])))
+             {struct idx}
+      : ilist2 (B := @id Type) headings[@idx].
+  Proof.
+    destruct idx; simpl in *;
+      revert tup; try revert idx;
+        pattern n0, headings; apply Vector.caseS.
+    - simpl; intros; exact tup.
+    - simpl; intros.
+      apply Tuple_DecomposeRawQueryStructure_Tuple_inj.
+      apply tup.
+  Defined.
+
+  Definition Tuple_DecomposeRawQueryStructure_inj'
+             {m : nat}
+             {qs_schema : RawQueryStructureSchema}
+             (schemaIdx : Fin.t _)
+             (attrIdx : Fin.t _)
+             (a : Vector.t Type m)
+             (a_inj : forall idx, Vector.nth a idx -> Vector.nth (AttrList (GetNRelSchemaHeading (qschemaSchemas qs_schema) schemaIdx)) attrIdx)
+             (idx : Fin.t m)
+             (tup : ilist2 (B := @id Type) (AttrList (GetNRelSchemaHeading (qschemaSchemas (DecomposeRawQueryStructureSchema qs_schema schemaIdx attrIdx a)) idx)))
+             (Tuple_inj :
+                ilist2 (B := @id Type) (AttrList (GetNRelSchemaHeading (qschemaSchemas (DecomposeRawQueryStructureSchema qs_schema schemaIdx attrIdx a)) idx))
+                ->
+                ilist2 (B := @id Type)
+     (DecomposeHeading attrIdx
+        (AttrList (GetNRelSchemaHeading (qschemaSchemas qs_schema) schemaIdx)) a)[@idx] := Tuple_DecomposeRawQueryStructure_Tuple_inj _ idx)
+    : ilist2 (B := @id Type) (AttrList (GetNRelSchemaHeading (qschemaSchemas qs_schema) schemaIdx)).
+    eapply Tuple_DecomposeHeading_inj; eauto.
+  Defined.
+
+    Fixpoint Tuple_DecomposeRawQueryStructure_Tuple_proj
+             {n m : nat}
+             (headings : _ )
+             (idx : Fin.t m)
+             (tup : ilist2 (B := @id Type) headings[@idx])
+             {struct idx}
+             :
+ilist2 (B := @id Type)
+          (AttrList
+             (rawSchemaHeading
+                (Vector.map
+                   (fun
+                      rawheading : t Type n =>
+                    {|
+                    rawSchemaHeading := {|
+                                        NumAttr := _;
+                                        AttrList := rawheading |};
+                    attrConstraints := None;
+                    tupleConstraints := None |})
+                   headings)[@idx]))
+          .
+  Proof.
+    destruct idx; simpl in *;
+      revert tup; try revert idx;
+        pattern n0, headings; apply Vector.caseS.
+    - simpl; intros; exact tup.
+    - simpl; intros.
+      apply Tuple_DecomposeRawQueryStructure_Tuple_proj.
+      apply tup.
+  Defined.
+
+  Definition Tuple_DecomposeRawQueryStructure_proj'
+             {m : nat}
+             {qs_schema : RawQueryStructureSchema}
+             (schemaIdx : Fin.t _)
+             (attrIdx : Fin.t _)
+             (a : Vector.t Type m)
+             (a_proj_index : Vector.nth (AttrList (GetNRelSchemaHeading (qschemaSchemas qs_schema) schemaIdx)) attrIdx -> Fin.t m)
+             (a_proj : forall (attr : Vector.nth _ attrIdx), a[@a_proj_index attr])
+             (tup : ilist2 (AttrList (GetNRelSchemaHeading (qschemaSchemas qs_schema) schemaIdx)))
+             (Tuple_proj :
+                ilist2 (B := @id Type)
+                       (DecomposeHeading attrIdx
+                                         (AttrList (GetNRelSchemaHeading (qschemaSchemas qs_schema) schemaIdx)) a)[@a_proj_index (GetAttributeRaw tup attrIdx)]
+                -> ilist2 (B := @id Type) (AttrList (GetNRelSchemaHeading (qschemaSchemas (DecomposeRawQueryStructureSchema qs_schema schemaIdx attrIdx a)) (a_proj_index (GetAttributeRaw tup attrIdx))))
+              := Tuple_DecomposeRawQueryStructure_Tuple_proj _ (a_proj_index _))
+    : ilist2 (B := @id Type) (AttrList (GetNRelSchemaHeading (qschemaSchemas (DecomposeRawQueryStructureSchema qs_schema schemaIdx attrIdx a)) (a_proj_index (GetAttributeRaw tup attrIdx)))).
+    eapply Tuple_proj; eapply Tuple_DecomposeHeading_proj; eauto.
+  Defined.
+
+  Definition DecomposeRawQueryStructureSchema_AbsR
+             {m : nat}
+             {qs_schema : RawQueryStructureSchema}
+             (schemaIdx : Fin.t _)
+             (attrIdx : Fin.t _)
+             (a : Vector.t Type m)
+             (a_proj_index : Vector.nth (AttrList (GetNRelSchemaHeading (qschemaSchemas qs_schema) schemaIdx)) attrIdx -> Fin.t m)
+             (a_proj : forall (attr : Vector.nth _ attrIdx), a[@a_proj_index attr])
+             (a_inj : forall idx, Vector.nth a idx -> Vector.nth (AttrList (GetNRelSchemaHeading (qschemaSchemas qs_schema) schemaIdx)) attrIdx)
+             (r_o : UnConstrQueryStructure qs_schema)
+             (r_n : UnConstrQueryStructure qs_schema * UnConstrQueryStructure (DecomposeRawQueryStructureSchema qs_schema schemaIdx attrIdx a))
+    : Prop :=
+    (forall Ridx, Same_set _ (GetUnConstrRelation r_o Ridx)
+                           (GetUnConstrRelation (fst r_n) Ridx))
+    /\ (forall Ridx tup,
+           IndexedEnsemble_In (GetUnConstrRelation (snd r_n) Ridx) tup
+           ->  IndexedEnsemble_In (GetUnConstrRelation (fst r_n) schemaIdx)
+                                  (Tuple_DecomposeRawQueryStructure_inj' _ _ a a_inj _ tup))
+    /\ (forall tup,
+           IndexedEnsemble_In (GetUnConstrRelation (fst r_n) schemaIdx) tup
+           -> IndexedEnsemble_In (GetUnConstrRelation (snd r_n) (a_proj_index (GetAttributeRaw tup attrIdx))) (Tuple_DecomposeRawQueryStructure_proj' _ _ a _ a_proj tup)).
+
+    Definition DecomposeRawQueryStructureSchema_AbsR'
+             {m : nat}
+             {qs_schema : QueryStructureSchema}
+             ( schemaIdx' : BoundedIndex (QSschemaNames qs_schema))
+             (schemaIdx := ibound (indexb schemaIdx'))
+             {attrIdx' : BoundedIndex (HeadingNames (QSGetNRelSchemaHeading (qs_schema) schemaIdx'))}
+             (attrIdx := ibound (indexb attrIdx'))
+             (attrIdx_inj : Fin.t _ -> Fin.t _)
+             (EnumTypes : Vector.t Type m)
+             (f' : Vector.nth (AttrList _) (attrIdx_inj attrIdx) -> SumType EnumTypes)
+             (f'' : SumType EnumTypes -> Vector.nth (AttrList _) (attrIdx_inj attrIdx))
+             (a_proj_index : Vector.nth (AttrList _) (attrIdx_inj attrIdx) -> Fin.t m :=
+                fun attr => SumType_index EnumTypes (f' attr))
+             (a_proj : forall (attr : Vector.nth _ (attrIdx_inj attrIdx)), EnumTypes[@a_proj_index attr] :=
+                fun attr => SumType_proj EnumTypes (f' attr))
+             (a_inj : forall idx, Vector.nth EnumTypes idx -> Vector.nth (AttrList _) (attrIdx_inj attrIdx) :=
+                fun idx attr => f'' (inj_SumType EnumTypes idx attr))
+             (r_o : UnConstrQueryStructure qs_schema)
+             (r_n : UnConstrQueryStructure qs_schema * UnConstrQueryStructure (DecomposeRawQueryStructureSchema qs_schema schemaIdx (attrIdx_inj attrIdx) EnumTypes))
+      : Prop :=
+      DecomposeRawQueryStructureSchema_AbsR (qs_schema := qs_schema)
+                                            schemaIdx (attrIdx_inj attrIdx)
+                                            EnumTypes a_proj_index a_proj a_inj r_o r_n.
+
+Definition DecomposeRawQueryStructureSchema_empty_AbsR
+             {m : nat}
+             {qs_schema : QueryStructureSchema}
+  : forall (schemaIdx : Fin.t _)
+           (attrIdx : Fin.t _)
+           (a : Vector.t Type m)
+           (a_proj_index : Vector.nth (AttrList (GetNRelSchemaHeading (qschemaSchemas qs_schema) schemaIdx)) attrIdx -> Fin.t m)
+           (a_proj : forall (attr : Vector.nth _ attrIdx), a[@a_proj_index attr])
+           (a_inj : forall idx, Vector.nth a idx -> Vector.nth (AttrList (GetNRelSchemaHeading (qschemaSchemas qs_schema) schemaIdx)) attrIdx),
+        DecomposeRawQueryStructureSchema_AbsR
+          schemaIdx attrIdx a a_proj_index a_proj a_inj
+          (DropQSConstraints (QSEmptySpec qs_schema))
+          (DropQSConstraints (QSEmptySpec qs_schema),
+           imap2 (fun ns : RawSchema => rawRel (RelationSchema:=ns))
+                 (Build_EmptyRelations
+                    (qschemaSchemas (DecomposeRawQueryStructureSchema qs_schema schemaIdx attrIdx a)))).
+Proof.
+  intros.
+  repeat split; simpl; intros; intuition.
+  - unfold GetUnConstrRelation in H.
+    rewrite <- ith_imap2,
+     EmptyRefinements.ith_Bounded_BuildEmptyRelations in H.
+    simpl in H; unfold IndexedEnsemble_In in H; destruct_ex;
+      inversion H.
+  - unfold GetUnConstrRelation, DropQSConstraints, QSEmptySpec in H.
+    rewrite <- ith_imap2 in H.
+    simpl in H.
+    rewrite EmptyRefinements.ith_Bounded_BuildEmptyRelations in H.
+    simpl in H; unfold IndexedEnsemble_In in H; destruct_ex;
+      inversion H.
+Qed.
+
+Definition DecomposeRawQueryStructureSchema_Insert_AbsR_neq
+             {m : nat}
+             {qs_schema : QueryStructureSchema}
+  : forall (schemaIdx : Fin.t _)
+           (attrIdx : Fin.t _)
+           (a : Vector.t Type m)
+           (a_proj_index : Vector.nth (AttrList (GetNRelSchemaHeading (qschemaSchemas qs_schema) schemaIdx)) attrIdx -> Fin.t m)
+           (a_proj : forall (attr : Vector.nth _ attrIdx), a[@a_proj_index attr])
+           (a_inj : forall idx, Vector.nth a idx -> Vector.nth (AttrList (GetNRelSchemaHeading (qschemaSchemas qs_schema) schemaIdx)) attrIdx)
+           r_o
+           r_n,
+    DecomposeRawQueryStructureSchema_AbsR
+      schemaIdx attrIdx a a_proj_index a_proj a_inj r_o r_n
+    ->
+    forall Ridx tup,
+      Ridx <> schemaIdx
+      -> DecomposeRawQueryStructureSchema_AbsR
+        schemaIdx attrIdx a a_proj_index a_proj a_inj
+        (UpdateUnConstrRelation r_o Ridx (EnsembleInsert tup (GetUnConstrRelation r_o Ridx)))
+        (UpdateUnConstrRelation (fst r_n) Ridx (EnsembleInsert tup (GetUnConstrRelation (fst r_n) Ridx)), snd r_n).
+Proof.
+  repeat split; simpl; intros.
+  - destruct (fin_eq_dec Ridx Ridx0); subst;
+      unfold GetUnConstrRelation, UpdateUnConstrRelation.
+    + rewrite !ith_replace2_Index_eq.
+      unfold Included; intros.
+      inversion H1; subst; intuition.
+      * econstructor; eauto.
+      * econstructor 2; eapply (proj1 H Ridx0); apply H2.
+    + rewrite !ith_replace2_Index_neq; eauto.
+      unfold Included; intros; eapply (proj1 H Ridx0); apply H1.
+  - destruct (fin_eq_dec Ridx Ridx0); subst;
+      unfold GetUnConstrRelation, UpdateUnConstrRelation.
+    + rewrite !ith_replace2_Index_eq.
+      unfold Included; intros.
+      inversion H1; subst; intuition.
+      * econstructor; eauto.
+      * econstructor 2; eapply (proj1 H Ridx0); apply H2.
+    + rewrite !ith_replace2_Index_neq; eauto.
+      unfold Included; intros; eapply (proj1 H Ridx0); apply H1.
+  - unfold GetUnConstrRelation, UpdateUnConstrRelation.
+    rewrite !ith_replace2_Index_neq; eauto.
+    eapply (proj2 H); eauto.
+  - unfold GetUnConstrRelation, UpdateUnConstrRelation in *.
+    rewrite !ith_replace2_Index_neq in H1; eauto.
+    eapply (proj2 H); eauto.
+Qed.
+
+Lemma Tuple_DecomposeRawQueryStructure_inj_inverse
+      {m : nat}
+      {qs_schema : QueryStructureSchema}
+  : forall (schemaIdx : Fin.t _)
+           (attrIdx : Fin.t _)
+           (a : Vector.t Type m)
+           (a_proj_index : Vector.nth (AttrList (GetNRelSchemaHeading (qschemaSchemas qs_schema) schemaIdx)) attrIdx -> Fin.t m)
+           (a_proj : forall (attr : Vector.nth _ attrIdx), a[@a_proj_index attr])
+           (a_inj : forall idx, Vector.nth a idx -> Vector.nth (AttrList (GetNRelSchemaHeading (qschemaSchemas qs_schema) schemaIdx)) attrIdx)
+           tup,
+    Tuple_DecomposeRawQueryStructure_inj' schemaIdx attrIdx a a_inj
+                                          (a_proj_index (GetAttributeRaw tup attrIdx))
+                                          (Tuple_DecomposeRawQueryStructure_proj' schemaIdx attrIdx a a_proj_index a_proj
+                                                                                 tup) = tup.
+Admitted.
+
+Definition DecomposeRawQueryStructureSchema_Insert_AbsR_eq
+             {m : nat}
+             {qs_schema : QueryStructureSchema}
+  : forall (schemaIdx : Fin.t _)
+           (attrIdx : Fin.t _)
+           (a : Vector.t Type m)
+           (a_proj_index : Vector.nth (AttrList (GetNRelSchemaHeading (qschemaSchemas qs_schema) schemaIdx)) attrIdx -> Fin.t m)
+           (a_proj : forall (attr : Vector.nth _ attrIdx), a[@a_proj_index attr])
+           (a_inj : forall idx, Vector.nth a idx -> Vector.nth (AttrList (GetNRelSchemaHeading (qschemaSchemas qs_schema) schemaIdx)) attrIdx)
+           r_o
+           r_n,
+    DecomposeRawQueryStructureSchema_AbsR
+      schemaIdx attrIdx a a_proj_index a_proj a_inj
+      r_o r_n
+    ->
+    forall tup,
+      DecomposeRawQueryStructureSchema_AbsR
+        schemaIdx attrIdx a a_proj_index a_proj a_inj
+        (UpdateUnConstrRelation r_o schemaIdx (EnsembleInsert tup (GetUnConstrRelation r_o schemaIdx)))
+        (UpdateUnConstrRelation (fst r_n) schemaIdx (EnsembleInsert tup (GetUnConstrRelation (fst r_n) schemaIdx)),
+         UpdateUnConstrRelation (snd r_n)
+                                (a_proj_index (GetAttributeRaw (indexedElement tup) attrIdx))
+                                (EnsembleInsert {| elementIndex := elementIndex tup;
+                                                   indexedElement :=
+                                                     Tuple_DecomposeRawQueryStructure_proj'
+                                                       _ _ _ _ a_proj
+                                                       (indexedElement tup) |} (GetUnConstrRelation (snd r_n) (a_proj_index (GetAttributeRaw (indexedElement tup) attrIdx))))).
+  repeat split; simpl; intros.
+  - destruct (fin_eq_dec schemaIdx Ridx); subst;
+      unfold GetUnConstrRelation, UpdateUnConstrRelation.
+    + rewrite !ith_replace2_Index_eq.
+      unfold Included; intros.
+      inversion H0; subst; intuition.
+      * econstructor; eauto.
+      * econstructor 2; eapply (proj1 H Ridx); apply H1.
+    + rewrite !ith_replace2_Index_neq; eauto.
+      unfold Included; intros; eapply (proj1 H Ridx); apply H0.
+  - destruct (fin_eq_dec schemaIdx Ridx); subst;
+      unfold GetUnConstrRelation, UpdateUnConstrRelation.
+    + rewrite !ith_replace2_Index_eq.
+      unfold Included; intros.
+      inversion H0; subst; intuition.
+      * econstructor; eauto.
+      * econstructor 2; eapply (proj1 H Ridx); apply H1.
+    + rewrite !ith_replace2_Index_neq; eauto.
+      unfold Included; intros; eapply (proj1 H Ridx); apply H0.
+  - unfold GetUnConstrRelation, UpdateUnConstrRelation in *.
+    + rewrite !ith_replace2_Index_eq in *.
+      simpl in H0.
+      destruct (fin_eq_dec
+                  Ridx
+                  (a_proj_index (GetAttributeRaw (indexedElement tup) attrIdx))); subst.
+      rewrite !ith_replace2_Index_eq in H0.
+      destruct H0 as [? [? | ?] ].
+      * destruct tup; injections; econstructor; econstructor.
+        f_equal; simpl.
+        apply Tuple_DecomposeRawQueryStructure_inj_inverse.
+      * destruct (proj1 (proj2 H) (a_proj_index (GetAttributeRaw (indexedElement tup) attrIdx)) tup0).
+        econstructor; eauto.
+        econstructor; econstructor 2; eauto.
+      * rewrite !ith_replace2_Index_neq in H0 by eauto.
+        destruct (proj1 (proj2 H) Ridx tup0 H0); eauto.
+        econstructor; econstructor 2; eauto.
+  - unfold GetUnConstrRelation, UpdateUnConstrRelation in *.
+    + rewrite !ith_replace2_Index_eq in H0.
+      destruct H0 as [? [? | ?] ]; subst.
+      * try rewrite !ith_replace2_Index_eq.
+        econstructor; econstructor; f_equal.
+      * destruct (proj2 (proj2 H) tup0).
+        econstructor; eauto.
+        simpl in *.
+        econstructor; simpl.
+        destruct tup; simpl in *.
+        clear r_o H H0 a_inj.
+        unfold In.
+        destruct (fin_eq_dec (a_proj_index (GetAttributeRaw tup0 attrIdx))
+                             (a_proj_index (GetAttributeRaw indexedElement attrIdx))
+                 ); subst;
+          [ | rewrite !ith_replace2_Index_neq; eauto].
+        match goal with
+          |- ith2 (replace_Index2 _ _ ?idx _) ?idx' _ =>
+          assert (idx = idx')
+        end.
+Admitted.
+
+Lemma UnConstrFreshIdx_Same_Set_Equiv {ElementType} :
+  forall (ensemble ensemble' : @IndexedEnsemble ElementType),
+    Same_set _ ensemble ensemble'
+    -> forall bound,
+      UnConstrFreshIdx ensemble bound
+      <-> UnConstrFreshIdx ensemble' bound.
+Proof.
+  unfold Same_set, UnConstrFreshIdx; intros.
+  intuition.
+  - eapply H; eapply H1; eauto.
+  - eapply H; eapply H0; eauto.
+Qed.
+
+Lemma refine_UnConstrFreshIdx_Same_Set_Equiv {ElementType} :
+  forall (ensemble ensemble' : @IndexedEnsemble ElementType),
+    Same_set _ ensemble ensemble'
+    -> refine {idx : nat | UnConstrFreshIdx ensemble idx}
+              {idx : nat | UnConstrFreshIdx ensemble' idx}.
+Proof.
+  intros.
+  unfold refine; intros; computes_to_inv; computes_to_econstructor.
+  rewrite UnConstrFreshIdx_Same_Set_Equiv; eauto.
+Qed.
+
+Corollary refine_UnConstrFreshIdx_DecomposeRawQueryStructureSchema_AbsR_Equiv
+  {m : nat}
+  {qs_schema : RawQueryStructureSchema}
+  (schemaIdx : Fin.t _)
+  (attrIdx : Fin.t _)
+  (a : Vector.t Type m)
+  (a_proj_index : Vector.nth (AttrList (GetNRelSchemaHeading (qschemaSchemas qs_schema) schemaIdx)) attrIdx -> Fin.t m)
+  (a_proj : forall (attr : Vector.nth _ attrIdx), a[@a_proj_index attr])
+  (a_inj : forall idx, Vector.nth a idx -> Vector.nth (AttrList (GetNRelSchemaHeading (qschemaSchemas qs_schema) schemaIdx)) attrIdx)
+  (r_o : UnConstrQueryStructure qs_schema)
+  (r_n : UnConstrQueryStructure qs_schema * UnConstrQueryStructure (DecomposeRawQueryStructureSchema qs_schema schemaIdx attrIdx a))
+  : DecomposeRawQueryStructureSchema_AbsR schemaIdx attrIdx a a_proj_index a_proj a_inj r_o r_n
+    -> forall Ridx,
+    refine {idx : nat | UnConstrFreshIdx (GetUnConstrRelation r_o Ridx) idx}
+           {idx : nat | UnConstrFreshIdx (GetUnConstrRelation (fst r_n) Ridx) idx}.
+Proof.
+  intros; apply refine_UnConstrFreshIdx_Same_Set_Equiv.
+  apply (proj1 H Ridx).
+Qed.
+
+Fixpoint Iterate_Equiv_QueryResultComp
+         m
+         {ResultT}
+         (heading : RawHeading)
+         (headings : Fin.t m -> RawHeading)
+         (Ensembles : forall (idx : Fin.t m),
+             @IndexedEnsemble (@RawTuple (headings idx)))
+         (inj_Tuple : forall (idx : Fin.t m),
+             @RawTuple (headings idx)
+             -> @RawTuple heading)
+         (body : @RawTuple heading -> Comp (list ResultT))
+         {struct m}
+  : Comp (list ResultT) :=
+  match m return
+        forall (headings : Fin.t m -> RawHeading),
+          (forall (idx : Fin.t m),
+              @IndexedEnsemble (@RawTuple (headings idx)))
+          -> (forall (idx : Fin.t m),
+                 @RawTuple (headings idx)
+                 -> @RawTuple heading)
+          -> Comp (list ResultT)
+         with
+         | 0 => fun _ _ _ => (ret List.nil)
+         | S m =>
+           fun headings Ensembles inj_Tuple =>
+             res <- QueryResultComp (Ensembles Fin.F1)
+                 (fun tup => body (inj_Tuple Fin.F1 tup));
+             res' <- Iterate_Equiv_QueryResultComp heading
+                  (fun idx => headings (Fin.FS idx))
+                  (fun idx => Ensembles (Fin.FS idx))
+                  (fun idx tup => (inj_Tuple (Fin.FS idx) tup))
+                  body
+             ;
+             ret (List.app res res')
+          end headings Ensembles inj_Tuple.
+
+Lemma refine_Iterate_Equiv_QueryResultComp
+  {m : nat}
+  {qs_schema : RawQueryStructureSchema}
+  {ResultT}
+  (schemaIdx : Fin.t _)
+  (body : @RawTuple _ -> Comp (list ResultT))
+  (attrIdx : Fin.t _)
+  (a : Vector.t Type m)
+  (a_proj_index : Vector.nth (AttrList (GetNRelSchemaHeading (qschemaSchemas qs_schema) schemaIdx)) attrIdx -> Fin.t m)
+  (a_proj : forall (attr : Vector.nth _ attrIdx), a[@a_proj_index attr])
+  (a_inj : forall idx, Vector.nth a idx -> Vector.nth (AttrList (GetNRelSchemaHeading (qschemaSchemas qs_schema) schemaIdx)) attrIdx)
+  (r_o : UnConstrQueryStructure qs_schema)
+  (r_n : UnConstrQueryStructure qs_schema * UnConstrQueryStructure (DecomposeRawQueryStructureSchema qs_schema schemaIdx attrIdx a))
+  : DecomposeRawQueryStructureSchema_AbsR schemaIdx attrIdx a a_proj_index a_proj a_inj r_o r_n
+    ->
+    refine (UnConstrQuery_In r_o schemaIdx body)
+           (Iterate_Equiv_QueryResultComp
+              _ _
+              (GetUnConstrRelation (snd r_n))
+              (Tuple_DecomposeRawQueryStructure_inj' _ _ a a_inj) body).
+Admitted.
+
+Arguments DecomposeRawQueryStructureSchema : simpl never.
+Arguments DecomposeRawQueryStructureSchema_AbsR : simpl never.
+Arguments inj_SumType : simpl never.
+Arguments inj_SumType : simpl never.
+Arguments SumType_proj : simpl never.
+Arguments SumType_index : simpl never.
+Arguments Vector.nth _ _ _ !_ / .
+
+Definition EnumIDs := ["A"; "NS"; "CNAME"; "SOA" ].
+Definition EnumID := BoundedString EnumIDs.
+Definition EnumTypes := [nat : Type; string : Type; nat : Type; list nat : Type].
+Definition EnumType := SumType EnumTypes.
+
+  Definition EESchema :=
+    Query Structure Schema
+          [ relation "foo" has
+                     schema <"A" :: nat, "BID" :: EnumID, "B" :: EnumType>
+            (*where (fun t => ibound (indexb t!"BID") = SumType_index _ t!"B" ) and (fun t t' => True) *);
+                    relation "bar" has
+                             schema <"C" :: nat, "D" :: list string>
+          ]
+          enforcing [ ].
+
+  Definition EESpec : ADT _ :=
+    Def ADT {
+          rep := QueryStructure EESchema,
+
+                 Def Constructor "Init" : rep := empty,,
+
+                                                      Def Method1 "AddData" (this : rep) (t : _) : rep * bool :=
+            Insert t into this!"foo",
+
+            Def Method1 "Process" (this : rep) (p : EnumID) : rep * list _ :=
+              results <- For (r in this!"foo")
+                      Where (r!"BID" = p)
+                      Return r;
+          ret (this, results)}.
+
+Definition EEImpl : FullySharpened EESpec.
+    unfold EESpec.
+    start sharpening ADT.
+    start_honing_QueryStructure'.
+    let AbsR' := constr:(@DecomposeRawQueryStructureSchema_AbsR' _ EESchema ``"foo" ``"B"
+                                                                id EnumTypes id id) in  hone representation using AbsR'.
+    {
+      simplify with monad laws.
+      apply refine_pick_val.
+      apply DecomposeRawQueryStructureSchema_empty_AbsR.
+    }
+    { (* Insert *)
+      unfold DecomposeRawQueryStructureSchema_AbsR' in *.
+      simpl in *; simplify with monad laws; cbv beta; simpl.
+      rewrite (refine_UnConstrFreshIdx_DecomposeRawQueryStructureSchema_AbsR_Equiv H0 Fin.F1).
+      unfold H; eapply refine_under_bind; intros.
+      apply refine_under_bind_both; intros.
+      apply refine_pick_val.
+      eapply (DecomposeRawQueryStructureSchema_Insert_AbsR_eq H0).
+      finish honing.
+    }
+    { (* Query *)
+      unfold DecomposeRawQueryStructureSchema_AbsR' in *.
+      simpl in *; simplify with monad laws; cbv beta; simpl.
+      rewrite refine_For; simplify with monad laws.
+      rewrite (refine_Iterate_Equiv_QueryResultComp _ H0).
+      simpl.
+      simplify with monad laws.
+      unfold Tuple_DecomposeRawQueryStructure_inj'.
+      simpl.
+      unfold GetAttributeRaw; simpl.
+      unfold icons2; simpl.
+      unfold ilist2_tl, ilist2_hd; simpl.
+      (* More refinements here. *)
+Abort.
+End DecomposeEnumField.
